deps/poulet4/lib/P4automata/Examples/SimpleSplitProofSmallInitLeap.v
@@ -7,6 +7,37 @@ Definition possibly_unsound_init_rel
     (mk_init 100 SimpleSplit.aut Simple.Start Split.StSplit1). 
 
 (*
+Ltac solve_bisim' :=
+  match goal with
+  | |- pre_bisimulation _ _ _ _ [] _ _ => apply PreBisimulationClose
+  | |- pre_bisimulation ?a ?wp _ ?R (?C :: _) _ _ =>
+    let H := fresh "H" in
+    assert (H: {R ⊨ C} + {~(R ⊨ C)})
+      by idtac;
+    destruct H;
+    [
+        let t := fresh "tmp" in
+        pose (t := wp a C); apply PreBisimulationExtend with (W := t);
+         [ reflexivity |  ]; compute in t; unfold t; clear t;
+         simpl (_ ++ _)
+  end
+*)
+
+
+Notation i := (separated _ _ _ SimpleSplit.aut).
+Notation "⟦ x ⟧" := (interp_crel i x).
+Notation "⦇ x ⦈" := (interp_conf_rel (a:=SimpleSplit.aut) x).
+Notation "R ⊨ q1 q2" := (⟦R⟧ q1 q2) (at level 40).
+Notation "R ⊨ S" := (forall q1 q2, ⟦R⟧ q1 q2 -> ⦇S⦈ q1 q2) (at level 40).
+
+Lemma forall_exists:
+  forall {A B} (P: A -> B -> Prop),
+  (exists x y, ~ P x y) ->
+  ~ (forall x y, P x y).
+Proof.
+  firstorder.
+Qed.
+
 Lemma prebisim_simple_split_sym_small_init_leap:
   pre_bisimulation SimpleSplit.aut
                    (WPSymLeap.wp (H:=SimpleSplit.header))
@@ -19,8 +50,83 @@ Proof.
   set (r := possibly_unsound_init_rel).
   cbv in r.
   subst r.
+  match goal with
+  | |- pre_bisimulation ?a ?wp _ ?R (?C :: _) _ _ =>
+    assert (~(R ⊨ C))
+  end.
+  {
+    repeat (unfold interp_crel,
+            interp_conf_rel,
+            interp_conf_state,
+            interp_store_rel,
+            interp_bit_expr,
+            interp_store_rel,
+            interp_state_template,
+            RelationClasses.relation_conjunction,
+            Relations.interp_rels,
+            separated
+            || cbn).
+    match goal with
+    | |- ~ (forall x y: ?T, @?Q x y) =>
+      eapply forall_exists with (P := Q)
+    end.
+    unfold P4automaton.configuration.
+    simpl.
+    unfold P4A.store, P4A.Env.t, Sum.H in *.
+    pose (l := [false;false;false;false;
+                false;false;false;false]).
+    assert (length l = 8) by reflexivity.
+    pose (t := Simple.Start).
+    pose (t' := Split.StSplit1).
+    pose (t'' := Split.StSplit2).
+    Import Tactics.
+    hfcrush.
+    Tactics.sfirstorder.
+    Hammer.hammer.
+    sfirstorder.
+    
+      idtac P;
+      eapply forall_exists; try eapply H
+    end.
+    Hammer.hammer.
+    do 2 destruct H0.
+    eapply H0.
+    specialize (H (inl (inl Simple.Start), [], [false;false;false;false;false;false;false;false]) (inr true, [], []));
+    intuition.
+             : {R ⊨ C} + {~(R ⊨ C)} 
+  match goal with
+  | |- pre_bisimulation ?a ?wp _ ?R (?C :: _) _ _ =>
+    let H := fresh "H" in
+    set (H := ltac:(
+                right;
+    repeat (unfold interp_crel,
+            interp_conf_rel,
+            interp_conf_state,
+            interp_store_rel,
+            interp_bit_expr,
+            interp_store_rel,
+            interp_state_template,
+            RelationClasses.relation_conjunction,
+            Relations.interp_rels,
+            separated
+            || cbn);
+    intuition;
+    simpl in *;
+    Hammer.hammer
+    specialize (H (inl (inl Simple.Start), [], [false;false;false;false;false;false;false;false]) (inr true, [], []));
+    intuition
+             )
+             : {R ⊨ C} + {~(R ⊨ C)} 
+        )
+  end.
+  eapply PreBisimulationExtend with (H0:=H); eauto.
+  exact I.
+  clear H.
+  cbn.
+  simpl (_ ++ _).
+  cbv.
+  solve_bisim'.
   time (repeat solve_bisim').
   cbv in *.
   intuition (try congruence).
 Qed.
-*)
